src/tls/test/TestRecord.fst
@@ -15,7 +15,7 @@ let hex_of_bytes = Platform.Bytes.hex_of_bytes
 
 let r = HyperHeap.root
 
-let fake_encode (pv: ProtocolVersion) (aeAlg: aeAlg) (key: string) (iv: string) (plain: string): bytes =
+let fake_aead (pv: ProtocolVersion) (aeAlg: aeAlg) (key: string) (iv: string) (plain: string): bytes =
   // AEAD_GCM.gid -> LHAEPlain.id -> TLSInfo.id
   let id = {
     msId = noMsId;
@@ -63,14 +63,70 @@ let fake_encode (pv: ProtocolVersion) (aeAlg: aeAlg) (key: string) (iv: string) 
 
   // StatefulLHAE.cipher -> StatefulPlain.cipher -> bytes
   // FIXME: without the three additional #-arguments below, extraction crashes
-  let c = encrypt #id #ad #rg w f in
+  StatefulLHAE.encrypt #id #ad #rg w f
 
-  c
+let fake_cbc (pv: ProtocolVersion) (aeAlg: aeAlg) (key: string) (iv: string) (plain: string) (macKey: string): bytes =
+  // TLSInfo.id
+  let id = {
+    msId = noMsId;
+    kdfAlg = PRF_SSL3_nested;
+    pv = pv;
+    aeAlg = aeAlg; // <- that's the relevant bit! the rest is dummy values 
+    csrConn = bytes_of_hex "";
+    ext = {
+      ne_extended_ms = false;
+      ne_extended_padding = false;
+      ne_secure_renegotiation = RI_Unsupported;
+      ne_supported_curves = None;
+      ne_supported_point_formats = None;
+      ne_server_names = None
+    };
+    writer = Client
+  } in
+
+  // ENC.encryptor -> ENC.state
+  let w: ENC.encryptor id =
+    let key: ENC.key id = bytes_of_hex key in
+    let log: HyperHeap.rref r _ = ralloc r Seq.createEmpty in
+    let state: ENC.localState r id =
+      let iv: ENC.iv id = bytes_of_hex iv in
+      ENC.OldBlockState id iv
+    in
+    let state: HyperHeap.rref r (ENC.localState r id) = ralloc r state in
+    ENC.StateB #id #Writer #r #r key state log
+  in
+
+  let text = bytes_of_hex plain in
+  // StatefulPlain.adata id -> bytes
+  let ad: StatefulPlain.adata id = StatefulPlain.makeAD id Content.Application_data in
+  // Range.frange -> Range.range
+  let rg: Range.frange id = 0, Platform.Bytes.length text in
+  // DataStream.fragment -> DataStream.pre_fragment -> bytes
+  let f: DataStream.fragment id rg = text |> unsafe_coerce in
+  // LHAEPlain.plain -> StatefulPlain.plain -> Content.fragment
+  let f: LHAEPlain.plain id ad rg = Content.CT_Data #id rg f |> unsafe_coerce in
+
+  let macKey = bytes_of_hex macKey in
+  ENC.enc id w ad rg f macKey
 
 let test_count = ref 0
 
-let one_test (pv: ProtocolVersion) (aeAlg: aeAlg) (key: string) (iv: string) (plain: string) (cipher: string) =
-  let output = fake_encode pv aeAlg key iv plain in
+let test_aead (pv: ProtocolVersion) (aeAlg: aeAlg) (key: string) (iv: string) (plain: string) (cipher: string) =
+  let output = fake_aead pv aeAlg key iv plain in
+  let output = hex_of_bytes output in
+  if output <> cipher then begin
+    IO.print_string ("Unexpected output: iv = " ^ iv ^ ", key = " ^ key ^
+        ", plain = " ^ plain ^ ", output = " ^ output ^ ", expected = " ^ cipher ^
+        "\n");
+    failwith "Error!"
+  end else begin
+    test_count := !test_count + 1;
+    let test_count = string_of_int !test_count in
+    IO.print_string ("Encryption test #" ^ test_count ^ ": OK\n")
+  end
+
+let test_cbc (pv: ProtocolVersion) (aeAlg: aeAlg) (key: string) (iv: string) (plain: string) (cipher: string) (macKey: string) =
+  let output = fake_cbc pv aeAlg key iv plain macKey in
   let output = hex_of_bytes output in
   if output <> cipher then begin
     IO.print_string ("Unexpected output: iv = " ^ iv ^ ", key = " ^ key ^
@@ -84,15 +140,16 @@ let one_test (pv: ProtocolVersion) (aeAlg: aeAlg) (key: string) (iv: string) (pl
   end
 
 let main () =
-  one_test TLS_1p2 (AEAD CoreCrypto.AES_128_GCM CoreCrypto.SHA256)
+  test_aead TLS_1p2 (AEAD CoreCrypto.AES_128_GCM CoreCrypto.SHA256)
     "152300c2dc44c8f695d4fb1471791659"
     "b56bf932"
     "474554202f20485454502f312e310d0a486f73743a20756e646566696e65640d0a0d0a"
     "0000000000000000ed3ca96c8bd2fbb376c2dc417f3ec249e8ab550dab1c421293f0e642a0c152b43a546a8b49b6128ee6e23454b7e580423ba985";
-  (* one_test TLS_1p2 (MtE (Block CoreCrypto.AES_128_CBC) CoreCrypto.SHA1)
+  test_cbc TLS_1p2 (MtE (Block CoreCrypto.AES_128_CBC) CoreCrypto.SHA1)
     "e77f6871e1697b2286416f973aee9ff6"
     "00000000000000000000000000000000"
     "474554202f20485454502f312e310d0a486f73743a20756e646566696e65640d0a0d0a"
-    "0000000000000000000000000000000028cf3b38da8358b78aae63e5fcc334c1eac5278a283fa709cb274df85a2a7fa21b767111bc7f73f37cb2697dbb41f903dd2a3e4470767f3cc5e2db1a2e781213"; *)
+    "0000000000000000000000000000000028cf3b38da8358b78aae63e5fcc334c1eac5278a283fa709cb274df85a2a7fa21b767111bc7f73f37cb2697dbb41f903dd2a3e4470767f3cc5e2db1a2e781213"
+    "431ad4d620ea0c63bf9afc8124afcae6729593f1";
   ()
 
